viper-total-heaps/TotalInternalConsistency.thy
@@ -94,67 +94,77 @@ lemma shift_up_preserves_loc_sum:
       and "nm_loc_sum loc nm s"
     shows "nm_loc_sum loc nm' s"
 proof -
-  from assms(1) obtain mh mp fnm pnm p mp' fnm' nm_sub where
+  from assms(1) obtain mh mp fnm pnm_opt p mp' fnm' nm'_sub where
     nm: "nm = NM mh mp fnm" and
-    pnm: "Some pnm = fnm (pred_id,vs)" and
+    pnm_opt: "pnm_opt = fnm (pred_id,vs)" and
     "p = mp (pred_id,vs)" and
     "q \<le> p" and
     "q \<noteq> 0" and
     "mp' = mp( (pred_id,vs) := p - q )" and
-    fnm': "fnm' = fnm( (pred_id,vs) := if q = p then None else Some (nested_mask_multiply pnm ((p - q) / p)) )" and
-    nm_sub: "nm_sub = NM mh mp' fnm'" and
-    nm': "nm' = nested_mask_merge nm_sub (nested_mask_multiply pnm (q / p))"
-    by (smt (verit, best) shift_up_simp)
-  have "fnm' (pred_id,vs) = None \<longleftrightarrow> q = p"
-    apply (cases "q = p")
-    by (simp add: fnm')+
-  from assms(2) obtain pf where
-    pf: "pf has_sumA (s - mh loc) \<and>
-         (\<forall>ploc. option_fold (\<lambda>m. nm_loc_sum loc m (pf ploc)) (pf ploc = 0) (fnm ploc))"
-    using nm nm_loc_sum.simps by blast
-  then obtain ps where pnm_sum: "nm_loc_sum loc pnm ps"
-    by (metis option_fold.simps(1) pnm)
-  with pf have "s - mh loc \<ge> ps"
-    by (metis all_pos has_sumA_nonneg_ge_one_preal nm_loc_sum_unique option_fold.simps(1) pnm)
-  hence "s \<ge> ps"
-    by (metis assms(2) nm nm_loc_sum.simps order.trans psub_smaller)
-
-  \<comment> \<open>sum of \<^term>\<open>nm_sub\<close>\<close>
-  from pnm_sum have "option_fold (\<lambda>nm. nm_loc_sum loc nm (ps * ((p - q) / p))) (ps * ((p - q) / p) = 0) (fnm' (pred_id,vs))"
-    apply (cases "fnm' (pred_id,vs)")
-     apply simp_all
-     apply (metis Rep_preal_inverse \<open>fnm' (pred_id, vs) = None \<longleftrightarrow> q = p\<close> cancel_comm_monoid_add_class.diff_cancel div_0 divide_preal.rep_eq minus_preal.rep_eq mult_not_zero zero_preal.rep_eq)
-    by (smt (verit, del_insts) \<open>q \<le> p\<close> all_pos divide_preal.rep_eq fnm' fun_upd_same less_eq_preal.rep_eq map_upd_eqD1 minus_preal.rep_eq mult_not_zero nm_loc_sum_mult nonzero_eq_divide_eq option.distinct(1) order_antisym pperm_pnone_pgt zero_preal.rep_eq)
-  moreover have "option_fold (\<lambda>nm. nm_loc_sum loc nm ps) (ps = 0) (fnm (pred_id,vs))"
-    by (metis option_fold.simps(1) pnm pnm_sum)
-  moreover have "fnm' = fnm( (pred_id, vs) := fnm' (pred_id, vs) )"
-    by (simp add: fnm')
-  ultimately have nm_sub_sum: "nm_loc_sum loc nm_sub (s - ps + ps * ((p - q) / p))"
-    using nm_loc_sum_change_sum[of loc mh mp fnm s ps "(pred_id,vs)" "ps * ((p - q) / p)" "fnm' (pred_id,vs)" mp'] nm assms(2) fnm' nm_sub
-    by argo
-
-  \<comment> \<open>sum of q/p of pnm\<close>
-  have pnm_frac_sum: "nm_loc_sum loc (nested_mask_multiply pnm (q / p)) (ps * (q / p))"
-    by (metis Rep_preal_inverse \<open>q \<le> p\<close> \<open>q \<noteq> pos_perm_class.pnone\<close> divide_eq_0_iff divide_preal.rep_eq leD nm_loc_sum_mult pnm_sum preal_not_0_gt_0 zero_preal.rep_eq)
-
-  \<comment> \<open>sum of nm'\<close>
-  have "s - ps + ps * ((p - q) / p) + ps * (q / p) = s"
-  proof -
-    have "s - ps + ps * ((p - q) / p) + ps * (q / p) = s - ps + (ps * ((p - q) / p) + ps * (q / p))"
-      using add.assoc by auto
-    moreover have "ps * ((p - q) / p) + ps * (q / p) = ps * ((p - q) / p + q / p)"
-      by (simp add: distrib_left)
-    moreover have "(p - q) / p + q / p = (p - q + q) / p"
-      by (simp add: PosReal.field_divide_inverse distrib_right)
-    moreover have "(p - q + q) / p = 1"
-      by (metis Rep_preal_inverse \<open>q \<le> p\<close> \<open>q \<noteq> pos_perm_class.pnone\<close> diff_add_cancel div_self divide_preal.rep_eq less_eq_preal.rep_eq minus_preal.rep_eq one_preal.rep_eq order_antisym plus_preal.rep_eq prat_non_negative zero_preal.rep_eq)
-    moreover have "s - ps + ps = s"
-      using greater_minus_plus \<open>ps \<le> s\<close> by auto
-    ultimately show ?thesis
-      by auto
+    fnm': "fnm' = fnm( (pred_id,vs) := nested_mask_multiply_option pnm_opt ((p - q) / p) )" and
+    nm_sub: "nm'_sub = NM mh mp' fnm'" and
+    nm': "Some nm' = nested_mask_merge_option (Some nm'_sub) (nested_mask_multiply_option pnm_opt (q / p))"
+    by (blast elim: shift_up.cases)
+  show ?thesis
+  proof (cases pnm_opt)
+    case None
+    then show ?thesis
+      by (metis assms(2) combine_options_simps(2) fnm' fun_upd_idem_iff nested_mask_merge_option.simps nested_mask_multiply_option.simps(1) nm nm' nm_loc_sum_mp_irrelevant nm_sub option.sel pnm_opt)
+  next
+    case (Some pnm)
+    have "fnm' (pred_id,vs) = None \<longleftrightarrow> q = p"
+      apply (cases "q = p")
+      using PosReal.field_divide_inverse Some fnm' minus_preal.abs_eq zero_preal_def
+       apply fastforce
+      by (metis Some \<open>q \<le> p\<close> comm_monoid_add_class.add_0 divide_eq_0_iff divide_preal.rep_eq fnm' fun_upd_def greater_minus_plus less_eq_preal.rep_eq linorder_not_le nested_mask_multiply_option.simps(2) not_None_eq preal_not_0_gt_0 zero_preal.rep_eq)
+    from assms(2) obtain pf where
+      pf: "pf has_sumA (s - mh loc) \<and>
+           (\<forall>ploc. option_fold (\<lambda>m. nm_loc_sum loc m (pf ploc)) (pf ploc = 0) (fnm ploc))"
+      using nm nm_loc_sum.simps by blast
+    then obtain ps where pnm_sum: "nm_loc_sum loc pnm ps"
+      by (metis option_fold.simps(1) pnm_opt Some)
+    with pf have "s - mh loc \<ge> ps"
+      by (metis all_pos has_sumA_nonneg_ge_one_preal nm_loc_sum_unique option_fold.simps(1) pnm_opt Some)
+    hence "s \<ge> ps"
+      by (metis assms(2) nm nm_loc_sum.simps order.trans psub_smaller)
+  
+    \<comment> \<open>sum of \<^term>\<open>nm_sub\<close>\<close>
+    from pnm_sum have "option_fold (\<lambda>nm. nm_loc_sum loc nm (ps * ((p - q) / p))) (ps * ((p - q) / p) = 0) (fnm' (pred_id,vs))"
+      apply (cases "fnm' (pred_id,vs)")
+       apply simp_all
+       apply (metis Rep_preal_inverse \<open>fnm' (pred_id, vs) = None \<longleftrightarrow> q = p\<close> cancel_comm_monoid_add_class.diff_cancel div_0 divide_preal.rep_eq minus_preal.rep_eq mult_not_zero zero_preal.rep_eq)
+      by (metis Some fnm' fun_upd_same is_none_simps(1) is_none_simps(2) nested_mask_multiply_option.simps(2) nm_loc_sum_mult option.sel preal_not_0_gt_0)
+    moreover have "option_fold (\<lambda>nm. nm_loc_sum loc nm ps) (ps = 0) (fnm (pred_id,vs))"
+      by (metis option_fold.simps(1) pnm_opt Some pnm_sum)
+    moreover have "fnm' = fnm( (pred_id, vs) := fnm' (pred_id, vs) )"
+      by (simp add: fnm')
+    ultimately have nm_sub_sum: "nm_loc_sum loc nm'_sub (s - ps + ps * ((p - q) / p))"
+      using nm_loc_sum_change_sum[of loc mh mp fnm s ps "(pred_id,vs)" "ps * ((p - q) / p)" "fnm' (pred_id,vs)" mp'] nm assms(2) fnm' nm_sub
+      by argo
+  
+    \<comment> \<open>sum of q/p of pnm\<close>
+    have pnm_frac_sum: "nm_loc_sum loc (nested_mask_multiply pnm (q / p)) (ps * (q / p))"
+      by (metis Rep_preal_inverse \<open>q \<le> p\<close> \<open>q \<noteq> pos_perm_class.pnone\<close> divide_eq_0_iff divide_preal.rep_eq leD nm_loc_sum_mult pnm_sum preal_not_0_gt_0 zero_preal.rep_eq)
+  
+    \<comment> \<open>sum of nm'\<close>
+    have "s - ps + ps * ((p - q) / p) + ps * (q / p) = s"
+    proof -
+      have "s - ps + ps * ((p - q) / p) + ps * (q / p) = s - ps + (ps * ((p - q) / p) + ps * (q / p))"
+        using add.assoc by auto
+      moreover have "ps * ((p - q) / p) + ps * (q / p) = ps * ((p - q) / p + q / p)"
+        by (simp add: distrib_left)
+      moreover have "(p - q) / p + q / p = (p - q + q) / p"
+        by (simp add: PosReal.field_divide_inverse distrib_right)
+      moreover have "(p - q + q) / p = 1"
+        by (metis Rep_preal_inverse \<open>q \<le> p\<close> \<open>q \<noteq> pos_perm_class.pnone\<close> diff_add_cancel div_self divide_preal.rep_eq less_eq_preal.rep_eq minus_preal.rep_eq one_preal.rep_eq order_antisym plus_preal.rep_eq prat_non_negative zero_preal.rep_eq)
+      moreover have "s - ps + ps = s"
+        using greater_minus_plus \<open>ps \<le> s\<close> by auto
+      ultimately show ?thesis
+        by auto
+    qed
+    thus "nm_loc_sum loc nm' s"
+      by (metis (no_types, lifting) Some add.right_neutral combine_options_simps(2) combine_options_simps(3) mult_not_zero nested_mask_merge_option.simps nested_mask_multiply_option.simps(2) nm' nm_loc_sum_add nm_sub_sum option.sel pnm_frac_sum)
   qed
-  thus "nm_loc_sum loc nm' s"
-    by (metis pnm_frac_sum nm_sub_sum nm' nm_loc_sum_add)
 qed
 
 
@@ -184,7 +194,7 @@ proof -
     \<omega>': "\<omega>' = \<lparr> get_store_total = get_store_total \<omega>,
                 get_trace_total = get_trace_total \<omega>,
                 get_total_full = add_to_nm_loc_total
-                  (add_to_mp_loc_total (get_total_full \<omega>1) (pred_id,vs) p)
+                  (inc_mp_loc_total (get_total_full \<omega>1) (pred_id,vs) p)
                   (pred_id,vs) nm_exh
               \<rparr>"
     using assms(1)
@@ -210,7 +220,7 @@ proof -
   ultimately have "s = s1 + s_exh"
     by (metis \<open>nm0 = get_nm_total_full \<omega>\<close> assms(2) nm_loc_sum_add nm_loc_sum_unique)
 
-  have "nm_loc_sum loc (get_nm_total (add_to_mp_loc_total (get_total_full \<omega>1) (pred_id,vs) p)) s1"
+  have "nm_loc_sum loc (get_nm_total (inc_mp_loc_total (get_total_full \<omega>1) (pred_id,vs) p)) s1"
     apply simp
     using \<open>nm_loc_sum loc nm1 s1\<close> nm1_def nm_loc_sum.elims(2) by fastforce
   hence "nm_loc_sum loc (get_nm_total_full \<omega>') (s1 + s_exh)"
